coq/Translation/TNNRCtoNNRCimp.v
@@ -1,0 +1,319 @@
+(*
+ * Copyright 2015-2016 IBM Corporation
+ *
+ * Licensed under the Apache License, Version 2.0 (the "License");
+ * you may not use this file except in compliance with the License.
+ * You may obtain a copy of the License at
+ *
+ * http://www.apache.org/licenses/LICENSE-2.0
+ *
+ * Unless required by applicable law or agreed to in writing, software
+ * distributed under the License is distributed on an "AS IS" BASIS,
+ * WITHOUT WARRANTIES OR CONDITIONS OF ANY KIND, either express or implied.
+ * See the License for the specific language governing permissions and
+ * limitations under the License.
+ *)
+
+Section TNNRCtoNNRCimp.
+  Require Import String.
+  Require Import List.
+  Require Import Bool.
+  Require Import Arith.
+  Require Import EquivDec.
+  Require Import Morphisms.
+  Require Import Permutation.
+  Require Import Eqdep_dec.
+  Require Import Program.
+  Require Import Utils.
+  Require Import CommonSystem.
+  Require Import cNNRCSystem.
+  Require Import NNRCSystem.
+  Require Import NNRCimpSystem.
+  Require Import NNRCtoNNRCimp.
+
+  Section from_stratified.
+
+    Context {m:basic_model}.
+    Context (τconstants:tbindings).
+
+    Local Open Scope nnrc_imp.
+
+    Definition pd_tbindings_lift (σ:tbindings) : pd_tbindings
+      := map_codomain Some σ.
+
+    Lemma lookup_pd_tbindings_lift Γ v :
+      lookup equiv_dec (pd_tbindings_lift Γ) v = lift Some (lookup equiv_dec Γ v).
+    Proof.
+      apply lookup_map_codomain.
+    Qed.
+
+    Lemma rproject_eq_preserves_sublist_full
+          {A} {odt:ODT}
+          (l1 l2 : list (string * A)) (sl : list string) :
+      is_list_sorted ODT_lt_dec (domain l1) = true ->
+      is_list_sorted ODT_lt_dec (domain l2) = true ->
+      sublist sl (domain l1) ->
+      rproject l1 sl = rproject l2 sl ->
+      sublist sl (domain l2).
+    Proof.
+      intros.
+      apply Sorted_incl_sublist.
+      - eapply is_list_sorted_Sorted_iff.
+        eapply is_list_sorted_sublist; try eapply H1.
+        eapply H.
+      - eapply is_list_sorted_Sorted_iff; eauto.
+      - intros.
+        assert (inn:In x (domain (rproject l1 sl))).
+        { apply rproject_domain_in; split; trivial.
+          eapply sublist_In; eauto.
+        }
+        rewrite H2 in inn.
+        apply rproject_domain_in in inn; tauto.
+    Qed.
+    
+    Lemma tnnrc_expr_to_nnrc_imp_expr_some_correct {e ei} :
+      nnrc_expr_to_nnrc_imp_expr e = Some ei ->
+      forall (Γc Γ:tbindings) (τ:rtype),
+        nnrc_type Γc Γ e τ <-> [ Γc ; pd_tbindings_lift Γ  ⊢ ei ▷ τ ].
+    Proof.
+      unfold nnrc_type.
+      Hint Constructors nnrc_core_type.
+      Hint Constructors nnrc_imp_expr_type.
+      
+      revert ei.
+      induction e; simpl; intros ei eqq Γc Γ τ; try discriminate.
+      - invcs eqq.
+        split; intros typ; invcs typ; eauto.
+      - invcs eqq.
+        split; intros typ; invcs typ; eauto.
+        + constructor.
+          rewrite lookup_pd_tbindings_lift.
+          rewrite H1; simpl; trivial.
+        + rewrite lookup_pd_tbindings_lift in H1.
+          apply some_lift in H1.
+          destruct H1 as [? ? eqq1]; invcs eqq1.
+          eauto.
+      - invcs eqq; split; intros typ; invcs typ; eauto.
+      - apply some_lift2 in eqq.
+        destruct eqq as [? [??[??]]]; subst.
+        split; intros typ; invcs typ
+        ; (econstructor; eauto 2
+           ; [eapply IHe1 | eapply IHe2]; eauto).        
+      - apply some_lift in eqq.
+        destruct eqq as [? ? ?]; subst.
+        split; intros typ; invcs typ
+        ; (econstructor; eauto 2
+           ; eapply IHe; eauto).        
+      - apply some_lift in eqq.
+        destruct eqq as [? ? ?]; subst.
+        split; intros typ.
+        + change (nnrc_type Γc Γ (NNRCGroupBy s l e) τ) in typ.
+          apply type_NNRCGroupBy_inv in typ.
+          destruct typ as [? [? [? [eqq1 [subl typ]]]]]; subst.
+          constructor; trivial.
+          apply IHe; eauto.
+        +  invcs typ.
+           change (nnrc_type Γc Γ (NNRCGroupBy s l e) (GroupBy_type s l k τl pf)).
+           apply type_NNRCGroupBy; trivial.
+           eapply IHe; eauto.
+    Qed.
+
+    Definition add_term_mc (term:terminator) τ (Δc:mc_tbindings)
+      := match term with
+         | Term_push x => (x,τ)::Δc
+         | Term_assign x => Δc
+         end.
+
+    Definition add_term_md (term:terminator) τ (Δd:md_tbindings)
+      := match term with
+         | Term_push x => Δd
+         | Term_assign x => (x,τ)::Δd
+         end.
+
+    Lemma terminate_type  {Γc:tbindings} {Γ:pd_tbindings} {e τ} :
+      [ Γc ; Γ  ⊢ e ▷ τ ] -> forall term Δc Δd  ,
+        [ Γc ; Γ , (add_term_mc term τ Δc) , (add_term_md term τ Δd) ⊢ terminate term e ].
+    Proof.
+      intros typ term Δc Δd.
+      destruct term; simpl
+      ; econstructor; simpl; try reflexivity; eauto
+      ; match_destr
+      ; congruence.
+    Qed.
+
+    Lemma nnrc_stmt_to_nnrc_imp_stmt_aux_must_assign
+          {fvs x s si} :
+      nnrc_stmt_to_nnrc_imp_stmt_aux fvs (Term_assign x) s = Some si ->
+      nnrc_imp_stmt_must_assign si x.
+    Proof.
+      revert x si.
+      induction s; simpl; intros x si eqq
+      ; repeat match_option_in eqq; invcs eqq; simpl; eauto.
+    Qed.
+    
+    Lemma tnnrc_stmt_to_nnrc_imp_stmt_aux_some_correct_fw {fvs term s si} :
+      nnrc_stmt_to_nnrc_imp_stmt_aux fvs term s = Some si ->
+      forall {Γc:tbindings} {Γ:tbindings} {τ:rtype},
+        nnrc_type Γc Γ s τ ->
+        forall Δc Δd,
+          [ Γc ; pd_tbindings_lift Γ , (add_term_mc term τ Δc) , (add_term_md term τ Δd) ⊢ si ].
+    Proof.
+      unfold nnrc_type.
+      Hint Resolve terminate_type.
+      Hint Constructors nnrc_core_type.
+      Hint Constructors nnrc_imp_expr_type.
+      intros eqq Γc.
+      revert fvs term si eqq.
+      induction s; simpl; intros fvs term si eqq Γ τ typ Δc Δd
+      ; repeat match_option_in eqq; invcs eqq; try solve [invcs typ; eauto 3].
+      - invcs typ.
+        apply terminate_type.
+        econstructor.
+        rewrite lookup_pd_tbindings_lift, H1; simpl; trivial.
+      - apply terminate_type.
+        apply (tnnrc_expr_to_nnrc_imp_expr_some_correct (e:=NNRCBinop b s1 s2))
+        ; simpl; eauto.
+      - apply terminate_type.
+        apply (tnnrc_expr_to_nnrc_imp_expr_some_correct (e:=NNRCUnop u s))
+        ; simpl; eauto.
+      - invcs typ.
+        econstructor.
+        + eapply nnrc_stmt_to_nnrc_imp_stmt_aux_must_assign; eauto.
+        + specialize (IHs1 _ _ _ eqq0 _ _ H4
+                           (add_term_mc term τ Δc)
+                           (add_term_md term τ Δd)); simpl in IHs1; eauto.
+        + specialize (IHs2 _ _ _ eqq1 _ _ H5); simpl in IHs2; eauto.
+      - invcs typ.
+        econstructor.
+        + econstructor.
+          * eapply tnnrc_expr_to_nnrc_imp_expr_some_correct; eauto.
+          * specialize (IHs2 _ _ _ eqq1 _ _ H5); simpl in IHs2; eauto.
+        + apply terminate_type.
+          econstructor; simpl.
+          match_destr; congruence.
+      - invcs typ.
+        econstructor; eauto.
+        apply (tnnrc_expr_to_nnrc_imp_expr_some_correct eqq0); trivial.
+      - invcs typ.
+        econstructor; eauto.
+        + apply (tnnrc_expr_to_nnrc_imp_expr_some_correct eqq0); eauto.
+        + specialize (IHs2 _ _ _ eqq1 _ _ H7); simpl in IHs2; eauto.
+        + specialize (IHs3 _ _ _ eqq2 _ _ H8); simpl in IHs3; eauto.
+      - apply terminate_type.
+        eapply (tnnrc_expr_to_nnrc_imp_expr_some_correct (e:= (NNRCGroupBy s l s0))); simpl; eauto.
+    Qed.
+
+
+    Theorem tnnrc_stmt_to_nnrc_imp_some_correct_fw {Γc:tbindings} {globals s si} :
+      nnrc_stmt_to_nnrc_imp globals s = Some si ->
+      forall {τ:rtype},
+        nnrc_type Γc nil s τ ->
+        [ h, Γc ⊢ si ▷ τ ].
+    Proof.
+      unfold nnrc_stmt_to_nnrc_imp, nnrc_imp_type; match_option
+      ; intros eqq1; invcs eqq1.
+      intros τ typ.
+      unfold nnrc_type in *.
+      apply (tnnrc_stmt_to_nnrc_imp_stmt_aux_some_correct_fw eqq typ).
+    Qed.
+
+    Definition get_terminator_type
+               (term:terminator)
+               (mc:mc_tbindings)
+               (md:md_tbindings) : option rtype :=
+      match term with
+      | Term_assign v => lookup equiv_dec md v
+      | Term_push v => lookup equiv_dec mc v
+      end.
+
+    Lemma terminate_type_inv  {Γc:tbindings} {Γ:pd_tbindings} {e τ} { term Δc Δd }:
+      [ Γc ; Γ , Δc , Δd ⊢ terminate term e ] ->
+      get_terminator_type term Δc Δd = Some τ ->
+      exists τ', [ Γc ; Γ  ⊢ e ▷ τ' ] /\ τ' ≤ τ.
+    Proof.
+      destruct term; simpl; intros typ eqq; invcs typ; simpl in *
+      ; unfold equiv_dec, string_eqdec in *
+      ; rewrite H5 in eqq; invcs eqq
+      ; eauto.
+    Qed.
+
+    Section counterexample.
+      Local Open Scope string.
+      
+      Example nnrc_stmt_with_weaker_nnrc_imp_type_example : nnrc 
+        := NNRCBinop (OpNatBinary NatPlus)
+                     (NNRCConst (dnat 1))
+                     (NNRCConst (dnat 2)).
+
+      Example nnrc_imp_of_nnrc_stmt_with_weaker_nnrc_imp_type_example
+        :=     (NNRCimpPush "x"
+                            (NNRCimpBinop (OpNatBinary NatPlus) (NNRCimpConst (dnat 1))
+                                          (NNRCimpConst (dnat 2)))).
+
+      Example nnrc_imp_of_nnrc_stmt_with_weaker_nnrc_imp_type_example_correct
+        : nnrc_stmt_to_nnrc_imp_stmt_aux nil (Term_push "x") nnrc_stmt_with_weaker_nnrc_imp_type_example = Some nnrc_imp_of_nnrc_stmt_with_weaker_nnrc_imp_type_example.
+      Proof.
+        vm_compute; reflexivity.
+      Qed.
+
+      Example nnrc_imp_typing_for_nnrc_with_weaker_nnrc_imp_type_example 
+        : [ nil ; pd_tbindings_lift nil , (add_term_mc (Term_push "x") ⊤ nil) , (add_term_md (Term_push "x") ⊤ nil) ⊢ nnrc_imp_of_nnrc_stmt_with_weaker_nnrc_imp_type_example ].
+      Proof.
+        unfold nnrc_imp_of_nnrc_stmt_with_weaker_nnrc_imp_type_example.
+        simpl.
+        econstructor; simpl.
+        - repeat econstructor.
+        - reflexivity.
+        - apply STop.
+      Qed.
+
+      Example nnrc_typing_for_nnrc_with_weaker_nnrc_imp_type_example 
+        : nnrc_type nil nil nnrc_stmt_with_weaker_nnrc_imp_type_example Nat.
+      Proof.
+        unfold nnrc_type, nnrc_stmt_with_weaker_nnrc_imp_type_example.
+        simpl.
+        econstructor; simpl
+        ; repeat econstructor.
+      Qed.
+
+      Example not_nnrc_typing_for_nnrc_with_weaker_nnrc_imp_type_example 
+        : ~ nnrc_type nil nil nnrc_stmt_with_weaker_nnrc_imp_type_example ⊤.
+      Proof.
+        unfold nnrc_type, nnrc_stmt_with_weaker_nnrc_imp_type_example
+        ; simpl; intros typ.
+        invcs typ.
+        invcs H3.
+      Qed.
+
+      Example nnrc_typing_weaker_nnrc_imp_translated_typing :
+        nnrc_stmt_to_nnrc_imp_stmt_aux nil (Term_push "x")
+                                       nnrc_stmt_with_weaker_nnrc_imp_type_example =
+        Some nnrc_imp_of_nnrc_stmt_with_weaker_nnrc_imp_type_example
+        /\ 
+        [ nil ; pd_tbindings_lift nil , (add_term_mc (Term_push "x") ⊤ nil) , (add_term_md (Term_push "x") ⊤ nil)
+                                                                                ⊢ nnrc_imp_of_nnrc_stmt_with_weaker_nnrc_imp_type_example ]
+        /\ ~ nnrc_type nil nil nnrc_stmt_with_weaker_nnrc_imp_type_example ⊤.
+      Proof.
+        split; [ | split].
+        - apply nnrc_imp_of_nnrc_stmt_with_weaker_nnrc_imp_type_example_correct.
+        - apply nnrc_imp_typing_for_nnrc_with_weaker_nnrc_imp_type_example.
+        - apply not_nnrc_typing_for_nnrc_with_weaker_nnrc_imp_type_example.
+      Qed.
+
+    (*
+    Example nnrc_with_weaker_nnrc_imp_type_example : nnrc 
+      := NNRCFor "x"%string (NNRCConst (dcoll (dnat 3:: dnat 4::dnat 5::nil)))
+                 nnrc_stmt_with_weaker_nnrc_imp_type_example.
+     *)
+
+    (* Backwards is more problematic, since the type system for nnrc_imp allows for 
+       free upcasts in a NNRCimpPush, whereas NNRC typing does not have
+       such a mechanism (and NNRC is not Proper with respect to subtyping, since
+       operators (such as (OpNatBinary NatPlus) are not.
+       For example, 
+       nnrc_typing_weaker_nnrc_imp_translated_typing witnesses a counter example.      *)
+    End counterexample.
+
+  End from_stratified.
+
+End TNNRCtoNNRCimp.
